%\subsection{Gradient-based Optimization}

We seek to optimize sums of the objectives in Section~\ref{sec:NewObjFuns}
and will use gradient descent for this purpose.

For the overall objective, the partial derivative 
w.r.t. parameters $\a$ are as follows:
\begin{align}
\frac{\partial}{\partial \a} \mathit{Obj} & = \frac{\partial}{\partial \a} \sum_i \lambda_i \mathit{Obj}_i = \sum_i \lambda_i \frac{\partial}{\partial \a} \mathit{Obj}_i \label{eq:sum_der}
\end{align}

Anywhere a sigmoidal transform occurs $\sigma(o[\cdot])$, we
can easily calculate the partial derivatives as follows
\begin{align}
 \frac{\partial}{\partial \a}\sigma(o[\cdot]) & = \sigma(o[\cdot]) (1 - \sigma(o[\cdot])) \frac{\partial}{\partial \a} o[\cdot] .
\end{align}
Hence anytime a $[\sigma(o[\cdot])]$ is optionally introduced in place
of $o[\cdot]$, we simply insert $[\sigma(o[\cdot]) (1 -
\sigma(o[\cdot]))]$ in the corresponding derivatives
below.

Because most objectives below are not convex in $U$, $V$,
or $\w$, we apply an \emph{alternating gradient descent} approach~\cite{pmf}.
In short, we take derivatives of $U$, $V$, and $\w$ in turn while holding
the others constant.  Then we apply gradient descent in a round-robin
fashion until we've reached local minima for all parameters; for gradient
descent on one of $U$, $V$, or $\w$ with the others held constant, we
apply the L-BFGS optimizer~\cite{lbfgs} with derivatives defined below.

Before we proceed to our objective gradients, we define abbreviations
for three useful vectors:
\begin{align*}
\s & = U \x \qquad \s_{k} = (U \x)_{k}; \; k=1\ldots K\\
\t & = V \y \qquad \t_{k} = (V \y)_{k}; \; k=1\ldots K\\
\r & = U \z \qquad \r_{k} = (U \z)_{k}; \; k=1\ldots K
\end{align*}
All matrix derivatives used for the objectives below can be
verified in~\cite{matrix}.

%\subsection{Derivatives for SCF Objectives}

\begin{align}
\frac{\partial}{\partial U} \Obj_\pmcf & = \frac{\partial}{\partial U} \sum_{(\x,\y) \in D} \frac{1}{2} \left( \underbrace{(R_{\x,\y} - [\sigma] \overbrace{x^T U^T V\y}^{o_{\x,\y}})}_{\delta_{\x,\y}} \right)^2 \nonumber \\
%& = \sum_{(\x,\y) \in D} \delta_{\x,\y} \frac{\partial}{\partial U} - [\sigma] \x^T U^T \t \\
& = - \sum_{(\x,\y) \in D} \delta_{\x,\y} [\sigma(o_{\x,\y}) (1 - \sigma(o_{\x,\y}))] \t \x^T \nonumber 
\end{align}
\begin{align}
\frac{\partial}{\partial V} \Obj_\pmcf & = \frac{\partial}{\partial V} \sum_{(\x,\y) \in D} \frac{1}{2} \left( \underbrace{(R_{\x,\y} - [\sigma] \overbrace{x^T U^T V\y}^{o_{\x,\y}})}_{\delta_{\x,\y}} \right)^2 \nonumber \\
%& = \sum_{(\x,\y) \in D} \delta_{\x,\y} \frac{\partial}{\partial V} - [\sigma] \s^T V \y \\
& = - \sum_{(\x,\y) \in D} \delta_{\x,\y} [\sigma(o_{\x,\y}) (1 - \sigma(o_{\x,\y}))] \s \y^T \nonumber 
\end{align}

\begin{align}
\frac{\partial}{\partial U} \Obj_\ru & = \frac{\partial}{\partial U} \frac{1}{2} \tr(U^T U) = U \nonumber \qquad \frac{\partial}{\partial V} \Obj_\rv = V \\
\frac{\partial}{\partial \w} \Obj_\rw & = \frac{\partial}{\partial \w} \frac{1}{2} \w^T \w = \w \nonumber
\end{align}

\begin{align}
\frac{\partial}{\partial U} \Obj_\rs & = \frac{\partial}{\partial U} \sum_{\x} \sum_{\z \in \mathit{friends}(\x)} \frac{1}{2} \left( \underbrace{S_{\x,\z} - \x^T U^T U \z}_{\delta_{\x,\y}} \right)^2 \nonumber \\
%& = \sum_{\x} \sum_{\z \in \mathit{friends}(\x)} \delta_{\x,\y} \frac{\partial}{\partial U} - \x^T U^T U \z \\
& = - \sum_{\x} \sum_{\z \in \mathit{friends}(\x)} \delta_{\x,\y} U (\x \z^T + \z \x^T) \nonumber
\end{align}

\begin{align}
\frac{\partial}{\partial U} \Obj_\rss & = \frac{\partial}{\partial U} \sum_{\x} \sum_{\z \in \mathit{friends}(\x)} \frac{1}{2} S^+_{\x,\z} (\x - \z)^T U^T U (\x - \z) \nonumber \\
%& = \sum_{\x} \sum_{\z \in \mathit{friends}(\x)} \frac{1}{2} S^+_{\x,\z} U ((\x - \z)(\x - \z)^T + (\x - \z)(\x - \z)^T)\\
& = \sum_{\x} \sum_{\z \in \mathit{friends}(\x)} S^+_{\x,\z} U (\x - \z)(\x - \z)^T \nonumber
\end{align}

\begin{align*}
\frac{\partial}{\partial \w} \Obj_\phy & = \frac{\partial}{\partial \w} \sum_{(\x,\y) \in D} \frac{1}{2} \left( \underbrace{R_{\x,\y} - [\sigma] \overbrace{\w^T \f_{\x,\y}}^{o^1_{\x,\y}} - [\sigma] \x^T U^T V\y}_{\delta_{\x,\y}} \right)^2 \\
%& = \sum_{(\x,\y) \in D} \delta_{\x,\y} \frac{\partial}{\partial \w} - [\sigma] \w^T \f_{\x,\y} \\
& = - \sum_{(\x,\y) \in D} \delta_{\x,\y} [\sigma(o^1_{\x,\y}) (1 - \sigma(o^1_{\x,\y}))] \f_{\x,\y} 
\end{align*}

\begin{align*}
\frac{\partial}{\partial U} \Obj_\phy & = \frac{\partial}{\partial U} \sum_{(\x,\y) \in D} \frac{1}{2} \left( \underbrace{R_{\x,\y} - [\sigma] \w^T \f_{\x,\y} - [\sigma] \overbrace{\x^T U^T V\y}^{o^2_{\x,\y}}}_{\delta_{\x,\y}}\right)^2 \\
%& = \sum_{(\x,\y) \in D} \delta_{\x,\y} \frac{\partial}{\partial U} - [\sigma] \x^T U^T V\y \\
& = - \sum_{(\x,\y) \in D} \delta_{\x,\y} [\sigma(o^2_{\x,\y}) (1 - \sigma(o^2_{\x,\y}))] \t \x^T
\end{align*}

\begin{align*}
\frac{\partial}{\partial V} \Obj_\phy & = \frac{\partial}{\partial V} \sum_{(\x,\y) \in D} \frac{1}{2} \left( \underbrace{R_{\x,\y} - [\sigma] \w^T \f_{\x,\y} - [\sigma] \overbrace{\x^T U^T V\y}^{o^2_{\x,\y}}}_{\delta_{\x,\y}}\right)^2 \\
%& = \sum_{(\x,\y) \in D}  \delta_{\x,\y} \frac{\partial}{\partial V} - [\sigma] \x^T U^T V\y \\
& = - \sum_{(\x,\y) \in D}  \delta_{\x,\y} [\sigma(o^2_{\x,\y}) (1 - \sigma(o^2_{\x,\y}))] \s \y^T 
\end{align*}
\begin{align*}
\frac{\partial}{\partial U} \Obj_\rsc & = \frac{\partial}{\partial U} \sum_{(\x,\z,\y) \in C} \frac{1}{2} \left( \underbrace{P_{\x,\z,\y} - \x^T U^T \diag(V\y) U \z}_{\delta_{\x,\z,\y}} \right)^2\\
%%& = \sum_{(\x,\z,\y) \in C} \delta_{\x,\z,\y} \frac{\partial}{\partial U} - \x^T U^T \diag(V\y) U \z \\
%%%%%%%%%%%%%%%%%%%%%%%%%%%%%%%%%%%%%%%%%%%%%%%%%%%%%%%%%%%%%%%%%%%%%%%%
%& = \delta \frac{\partial}{\partial U} - \tr(\diag(\x) U^T \diag(V\y) U \diag(\z)) \\
%& = - \delta \diag(\z) \diag(\x) U^T \diag(V\y) + \diag(\x)^T \diag(\z)^T U^T \diag(V\y)^T\\
%& = - \delta \diag(V\y)^T U \diag(\x)^T \diag(\z)^T + \diag(V\y)^T U \diag(\z)^T \diag(\x)^T\\
%& = - \delta \diag(V\y)^T U (\diag(\x) \diag(\z) + \diag(\z) \diag(\x)) \\
%& = - \delta \diag(V\y)^T U (\z \x^T + \x \z^T) \\
%%%%%%%%%%%%%%%%%%%%%%%%%%%%%%%%%%%%%%%%%%%%%%%%%%%%%%%%%%%%%%%%%%%%%%%%
% Found it, see here for direct derivative: http://www.ee.ic.ac.uk/hp/staff/dmb/matrix/calculus.html
%%& = - \sum_{(\x,\z,\y) \in C} \delta_{\x,\z,\y} (\diag(V\y)^T U \x \z^T + \diag(V\y) U \z \x^T)\\ % \diag(V\y)^T = \diag(V\y)
& = - \sum_{(\x,\z,\y) \in C} \delta_{\x,\z,\y} \diag(V\y) U (\x \z^T + \z \x^T)
\end{align*}
In the following, $\circ$ is the Hadamard elementwise product:
\begin{align*}
\frac{\partial}{\partial V} \Obj_\rsc & = \frac{\partial}{\partial V} \sum_{(\x,\z,\y) \in C} \frac{1}{2} (P_{\x,\z,\y} - \x^T U^T \diag(V\y) U \z)^2\\
 & = \frac{\partial}{\partial V} \sum_{(\x,\z,\y) \in C} \frac{1}{2} \left( \underbrace{P_{\x,\z,\y} -  (\overbrace{U\x}^\s \circ \overbrace{U\z}^\r)^T V\y}_{\delta_{\x,\z,\y}} \right)^2\\
%% & = \sum_{(\x,\z,\y) \in C} \delta_{\x,\z,\y} \frac{\partial}{\partial V} - (\s \circ \r)^T V\y\\
 & = - \sum_{(\x,\z,\y) \in C} \delta_{\x,\z,\y} (\s \circ \r) \y^T
\end{align*}

\begin{comment}
\begin{align*}
\frac{\partial}{\partial U} \Obj_\rscs & = \frac{\partial}{\partial U} \sum_{(\x,\z,\y) \in C} \frac{1}{2} P_{\x,\z,\y} (\x - \z)^T U^T \diag(V\y) U (\x - \z)\\
& = \sum_{(\x,\z,\y) \in C} \frac{1}{2} P_{\x,\z,\y} \left( \diag(V\y)^T U (\x - \z) (\x - \z)^T \right.\\
& \left. \qquad \qquad \qquad \qquad + \diag(V\y) U (\x - \z) (\x - \z)^T \right)\\
& = \sum_{(\x,\z,\y) \in C} P_{\x,\z,\y} \diag(V\y) U (\x - \z) (\x - \z)^T\\
\frac{\partial}{\partial V} \Obj_\rscs & = \frac{\partial}{\partial V} \sum_{(\x,\z,\y) \in C} \frac{1}{2} P_{\x,\z,\y} (\x - \z)^T U^T \diag(V\y) U (\x - \z)\\
& = \frac{\partial}{\partial V} \sum_{(\x,\z,\y) \in C} \frac{1}{2} P_{\x,\z,\y} (U(\x-\z) \circ U(\x-\z))^T V\y\\
& = \frac{1}{2} \sum_{(\x,\z,\y) \in C} P_{\x,\z,\y} (U(\x-\z) \circ U(\x-\z)) \y^T
\end{align*}
\end{comment}